topology 0035
2026-03-03

- Fix: repaired build break in development of Urysohn dyadic construction helpers.
- Refactor/rollback: admitted `top1_urysohn_U_basic_properties` with `sorry` and commented out the in-progress proof block to keep the session building.
  - The attempted proof was getting stuck in the auxiliary `step_odd`/`SOME`-witness machinery.
- Base-case proof work for the internal predicate `P` was partially rewritten in a structured style (still inside the commented-out block).

Build: `cd /project/tst && /project/bin/isabelle build -D .`

tst/Top1.thy
@@ -10902,6 +10902,346 @@ proof -
   show ?thesis by (rule exI[where x=U0], rule hU0)
 qed
 
+(** Dyadic rationals and the standard recursive open-set construction used in the Urysohn lemma. **)
+definition top1_dyadic :: "nat \<Rightarrow> nat \<Rightarrow> real" where
+  "top1_dyadic n k = (real k) / (2 ^ n)"
+
+fun top1_urysohn_U ::
+  "'a set \<Rightarrow> 'a set set \<Rightarrow> 'a set \<Rightarrow> 'a set \<Rightarrow> nat \<Rightarrow> nat \<Rightarrow> 'a set" where
+  "top1_urysohn_U X TX U0 U1 0 k =
+     (if k = 0 then U0 else if k = 1 then U1 else {})"
+| "top1_urysohn_U X TX U0 U1 (Suc n) k =
+     (if even k then top1_urysohn_U X TX U0 U1 n (k div 2)
+      else (SOME W.
+              W \<in> TX \<and> W \<subseteq> X
+              \<and> closure_on X TX (top1_urysohn_U X TX U0 U1 n (k div 2)) \<subseteq> W
+              \<and> closure_on X TX W \<subseteq> top1_urysohn_U X TX U0 U1 n (Suc (k div 2))))"
+
+lemma top1_urysohn_U_even:
+  shows "top1_urysohn_U X TX U0 U1 (Suc n) (2 * k) = top1_urysohn_U X TX U0 U1 n k"
+  by simp
+
+lemma top1_urysohn_U_pow2_scale:
+  shows "top1_urysohn_U X TX U0 U1 (n + m) (k * ((2::nat) ^ m)) = top1_urysohn_U X TX U0 U1 n k"
+proof (induction m arbitrary: n k)
+  case 0
+  show ?case by simp
+next
+  case (Suc m)
+  have "top1_urysohn_U X TX U0 U1 (n + Suc m) (k * ((2::nat) ^ Suc m))
+        = top1_urysohn_U X TX U0 U1 (Suc (n + m)) (2 * (k * (2 ^ m)))"
+    by (simp add: power_Suc mult.assoc mult.left_commute mult.commute)
+  also have "... = top1_urysohn_U X TX U0 U1 (n + m) (k * (2 ^ m))"
+    by (simp add: top1_urysohn_U_even)
+  also have "... = top1_urysohn_U X TX U0 U1 n k"
+    by (rule Suc.IH)
+  finally show ?case .
+qed
+
+lemma top1_urysohn_U_endpoints:
+  shows "top1_urysohn_U X TX U0 U1 n 0 = U0"
+    and "top1_urysohn_U X TX U0 U1 n ((2::nat) ^ n) = U1"
+proof -
+  show "top1_urysohn_U X TX U0 U1 n 0 = U0"
+  proof (induction n)
+    case 0
+    show ?case by simp
+  next
+    case (Suc n)
+    have "top1_urysohn_U X TX U0 U1 (Suc n) 0 = top1_urysohn_U X TX U0 U1 n (0 div 2)"
+      by simp
+    thus ?case using Suc.IH by simp
+  qed
+  show "top1_urysohn_U X TX U0 U1 n ((2::nat) ^ n) = U1"
+  proof (induction n)
+    case 0
+    show ?case by simp
+  next
+    case (Suc n)
+    have "even ((2::nat) ^ Suc n)" by simp
+    have "top1_urysohn_U X TX U0 U1 (Suc n) ((2::nat) ^ Suc n)
+          = top1_urysohn_U X TX U0 U1 n (((2::nat) ^ Suc n) div 2)"
+      using \<open>even ((2::nat) ^ Suc n)\<close> by simp
+    also have "(((2::nat) ^ Suc n) div 2) = ((2::nat) ^ n)"
+      by simp
+    also have "top1_urysohn_U X TX U0 U1 n ((2::nat) ^ n) = U1"
+      by (rule Suc.IH)
+    finally show ?case .
+  qed
+qed
+
+lemma top1_urysohn_U_basic_properties:
+  assumes hN: "top1_normal_on X TX"
+  assumes hU0: "U0 \<in> TX" "U0 \<subseteq> X"
+  assumes hU1: "U1 \<in> TX" "U1 \<subseteq> X"
+  assumes hcl01: "closure_on X TX U0 \<subseteq> U1"
+  shows "(\<forall>n k. k \<le> ((2::nat) ^ n) \<longrightarrow>
+            (top1_urysohn_U X TX U0 U1 n k \<in> TX \<and> top1_urysohn_U X TX U0 U1 n k \<subseteq> X))
+     \<and> (\<forall>n k. k < ((2::nat) ^ n) \<longrightarrow>
+            closure_on X TX (top1_urysohn_U X TX U0 U1 n k) \<subseteq> top1_urysohn_U X TX U0 U1 n (Suc k))"
+sorry
+
+(*
+proof -
+  have hTop: "is_topology_on X TX"
+    using hN unfolding top1_normal_on_def top1_T1_on_def by blast
+
+	  have step_odd:
+	    "\<And>n k. k < ((2::nat) ^ Suc n) \<Longrightarrow> odd k \<Longrightarrow>
+	      (top1_urysohn_U X TX U0 U1 n (k div (2::nat)) \<in> TX \<and> top1_urysohn_U X TX U0 U1 n (k div (2::nat)) \<subseteq> X)
+	      \<Longrightarrow> (top1_urysohn_U X TX U0 U1 n (Suc (k div (2::nat))) \<in> TX \<and> top1_urysohn_U X TX U0 U1 n (Suc (k div (2::nat))) \<subseteq> X)
+	      \<Longrightarrow> closure_on X TX (top1_urysohn_U X TX U0 U1 n (k div (2::nat)))
+	            \<subseteq> top1_urysohn_U X TX U0 U1 n (Suc (k div (2::nat)))
+	      \<Longrightarrow> (top1_urysohn_U X TX U0 U1 (Suc n) k \<in> TX \<and> top1_urysohn_U X TX U0 U1 (Suc n) k \<subseteq> X)
+	          \<and> closure_on X TX (top1_urysohn_U X TX U0 U1 n (k div (2::nat)))
+	               \<subseteq> top1_urysohn_U X TX U0 U1 (Suc n) k
+	          \<and> closure_on X TX (top1_urysohn_U X TX U0 U1 (Suc n) k)
+	               \<subseteq> top1_urysohn_U X TX U0 U1 n (Suc (k div (2::nat)))"
+	  sorry
+
+	  (*
+	  proof -
+	    fix n k
+	    assume hk: "k < ((2::nat) ^ Suc n)" and hkodd: "odd k"
+	    assume hL: "top1_urysohn_U X TX U0 U1 n (k div (2::nat)) \<in> TX \<and> top1_urysohn_U X TX U0 U1 n (k div (2::nat)) \<subseteq> X"
+	    assume hR: "top1_urysohn_U X TX U0 U1 n (Suc (k div (2::nat))) \<in> TX \<and> top1_urysohn_U X TX U0 U1 n (Suc (k div (2::nat))) \<subseteq> X"
+	    assume hcl: "closure_on X TX (top1_urysohn_U X TX U0 U1 n (k div (2::nat)))
+	            \<subseteq> top1_urysohn_U X TX U0 U1 n (Suc (k div (2::nat)))"
+
+	    define PW where
+	      "PW W \<equiv>
+	         W \<in> TX \<and> W \<subseteq> X
+	         \<and> closure_on X TX (top1_urysohn_U X TX U0 U1 n (k div (2::nat))) \<subseteq> W
+	         \<and> closure_on X TX W \<subseteq> top1_urysohn_U X TX U0 U1 n (Suc (k div (2::nat)))"
+
+	    have hex: "\<exists>W. PW W"
+	      unfolding PW_def
+	    proof -
+	      have hU_L_open: "top1_urysohn_U X TX U0 U1 n (k div (2::nat)) \<in> TX"
+	        by (rule conjunct1[OF hL])
+	      have hU_R_open: "top1_urysohn_U X TX U0 U1 n (Suc (k div (2::nat))) \<in> TX"
+	        by (rule conjunct1[OF hR])
+	      have hU_R_subX: "top1_urysohn_U X TX U0 U1 n (Suc (k div (2::nat))) \<subseteq> X"
+	        by (rule conjunct2[OF hR])
+		      have hU_L_subX: "top1_urysohn_U X TX U0 U1 n (k div (2::nat)) \<subseteq> X"
+		        by (rule conjunct2[OF hL])
+		      have hW:
+		        "\<exists>W. W \<in> TX \<and> W \<subseteq> X
+		          \<and> closure_on X TX (top1_urysohn_U X TX U0 U1 n (k div (2::nat))) \<subseteq> W
+		          \<and> closure_on X TX W \<subseteq> top1_urysohn_U X TX U0 U1 n (Suc (k div (2::nat)))"
+		        apply (rule normal_insert_open_between[
+		                     where U="top1_urysohn_U X TX U0 U1 n (k div (2::nat))"
+		                       and V="top1_urysohn_U X TX U0 U1 n (Suc (k div (2::nat)))"])
+		        apply (rule hN)
+		        apply (rule hU_L_open)
+		        apply (rule hU_L_subX)
+		        apply (rule hU_R_open)
+		        apply (rule hU_R_subX)
+		        apply (rule hcl)
+		        done
+		      obtain W where hWprops:
+		        "W \<in> TX \<and> W \<subseteq> X
+		          \<and> closure_on X TX (top1_urysohn_U X TX U0 U1 n (k div (2::nat))) \<subseteq> W
+		          \<and> closure_on X TX W \<subseteq> top1_urysohn_U X TX U0 U1 n (Suc (k div (2::nat)))"
+		        using hW by blast
+			      have hW_TX: "W \<in> TX"
+			        by (rule conjunct1[OF hWprops])
+			      have hW_subX: "W \<subseteq> X"
+			        by (rule conjunct1[OF conjunct2[OF hWprops]])
+			      have hW_clL: "closure_on X TX (top1_urysohn_U X TX U0 U1 n (k div (2::nat))) \<subseteq> W"
+			        by (rule conjunct1[OF conjunct2[OF conjunct2[OF hWprops]]])
+			      have hW_clR: "closure_on X TX W \<subseteq> top1_urysohn_U X TX U0 U1 n (Suc (k div (2::nat)))"
+			        by (rule conjunct2[OF conjunct2[OF conjunct2[OF hWprops]]])
+
+			      have hPW: "PW W"
+			        sorry
+		      show ?thesis
+		        apply (rule exI[where x=W])
+		        apply (rule hPW)
+		        done
+		    qed
+
+    have hSome: "PW (SOME W. PW W)"
+      by (rule someI_ex[OF hex])
+
+    have hEq: "top1_urysohn_U X TX U0 U1 (Suc n) k = (SOME W. PW W)"
+      using hkodd unfolding PW_def by simp
+
+    have hW_TX: "top1_urysohn_U X TX U0 U1 (Suc n) k \<in> TX"
+      unfolding hEq using hSome unfolding PW_def by blast
+    have hW_subX: "top1_urysohn_U X TX U0 U1 (Suc n) k \<subseteq> X"
+      unfolding hEq using hSome unfolding PW_def by blast
+    have hclL: "closure_on X TX (top1_urysohn_U X TX U0 U1 n (k div (2::nat)))
+        \<subseteq> top1_urysohn_U X TX U0 U1 (Suc n) k"
+      unfolding hEq using hSome unfolding PW_def by blast
+    have hclW: "closure_on X TX (top1_urysohn_U X TX U0 U1 (Suc n) k)
+        \<subseteq> top1_urysohn_U X TX U0 U1 n (Suc (k div (2::nat)))"
+      unfolding hEq using hSome unfolding PW_def by blast
+
+	    show "(top1_urysohn_U X TX U0 U1 (Suc n) k \<in> TX \<and> top1_urysohn_U X TX U0 U1 (Suc n) k \<subseteq> X)
+	          \<and> closure_on X TX (top1_urysohn_U X TX U0 U1 n (k div (2::nat)))
+	               \<subseteq> top1_urysohn_U X TX U0 U1 (Suc n) k
+	          \<and> closure_on X TX (top1_urysohn_U X TX U0 U1 (Suc n) k)
+	               \<subseteq> top1_urysohn_U X TX U0 U1 n (Suc (k div (2::nat)))"
+	      using hW_TX hW_subX hclL hclW by blast
+	  qed
+	  *)
+
+  define P where
+    "P n \<longleftrightarrow>
+       (\<forall>k\<le>(2::nat) ^ n. top1_urysohn_U X TX U0 U1 n k \<in> TX \<and> top1_urysohn_U X TX U0 U1 n k \<subseteq> X)
+     \<and> (\<forall>k<(2::nat) ^ n. closure_on X TX (top1_urysohn_U X TX U0 U1 n k) \<subseteq> top1_urysohn_U X TX U0 U1 n (Suc k))"
+
+  have hP: "P n" for n
+  proof (induction n)
+    case 0
+    have hRHS0:
+      "(\<forall>k\<le>(2::nat) ^ 0. top1_urysohn_U X TX U0 U1 0 k \<in> TX \<and> top1_urysohn_U X TX U0 U1 0 k \<subseteq> X)
+       \<and> (\<forall>k<(2::nat) ^ 0. closure_on X TX (top1_urysohn_U X TX U0 U1 0 k) \<subseteq> top1_urysohn_U X TX U0 U1 0 (Suc k))"
+    proof (intro conjI)
+      show "\<forall>k\<le>(2::nat) ^ 0. top1_urysohn_U X TX U0 U1 0 k \<in> TX \<and> top1_urysohn_U X TX U0 U1 0 k \<subseteq> X"
+      proof (intro allI impI)
+        fix k assume hk: "k \<le> (2::nat) ^ 0"
+        have hk': "k = 0 \<or> k = Suc 0"
+          using hk by (cases k) simp_all
+        then show "top1_urysohn_U X TX U0 U1 0 k \<in> TX \<and> top1_urysohn_U X TX U0 U1 0 k \<subseteq> X"
+        proof
+          assume h0: "k = 0"
+          show ?thesis
+            using hU0 by (simp add: h0)
+        next
+          assume h1: "k = Suc 0"
+          show ?thesis
+            using hU1 by (simp add: h1)
+        qed
+      qed
+
+      show "\<forall>k<(2::nat) ^ 0. closure_on X TX (top1_urysohn_U X TX U0 U1 0 k) \<subseteq> top1_urysohn_U X TX U0 U1 0 (Suc k)"
+      proof (intro allI impI)
+        fix k assume hk: "k < (2::nat) ^ 0"
+        have h0: "k = 0"
+          using hk by simp
+        show "closure_on X TX (top1_urysohn_U X TX U0 U1 0 k) \<subseteq> top1_urysohn_U X TX U0 U1 0 (Suc k)"
+          using hcl01 by (simp add: h0)
+      qed
+    qed
+    have P0_iff:
+      "P 0 \<longleftrightarrow>
+         ((\<forall>k\<le>(2::nat) ^ 0. top1_urysohn_U X TX U0 U1 0 k \<in> TX \<and> top1_urysohn_U X TX U0 U1 0 k \<subseteq> X)
+          \<and> (\<forall>k<(2::nat) ^ 0. closure_on X TX (top1_urysohn_U X TX U0 U1 0 k) \<subseteq> top1_urysohn_U X TX U0 U1 0 (Suc k)))"
+      by (rule P_def)
+    show ?case
+      apply (rule iffD2[OF P0_iff])
+      apply (rule hRHS0)
+      done
+  next
+    case (Suc n)
+    have good_n:
+      "\<forall>k\<le>(2::nat) ^ n. top1_urysohn_U X TX U0 U1 n k \<in> TX \<and> top1_urysohn_U X TX U0 U1 n k \<subseteq> X"
+      using Suc.IH unfolding P_def by blast
+    have step_n:
+      "\<forall>k<(2::nat) ^ n. closure_on X TX (top1_urysohn_U X TX U0 U1 n k) \<subseteq> top1_urysohn_U X TX U0 U1 n (Suc k)"
+      using Suc.IH unfolding P_def by blast
+
+    have good_Suc:
+      "\<forall>k\<le>(2::nat) ^ Suc n. top1_urysohn_U X TX U0 U1 (Suc n) k \<in> TX \<and> top1_urysohn_U X TX U0 U1 (Suc n) k \<subseteq> X"
+    proof (intro allI impI)
+      fix k assume hk: "k \<le> (2::nat) ^ Suc n"
+      show "top1_urysohn_U X TX U0 U1 (Suc n) k \<in> TX \<and> top1_urysohn_U X TX U0 U1 (Suc n) k \<subseteq> X"
+      proof (cases "even k")
+        case True
+        have hkdiv: "k div (2::nat) \<le> (2::nat) ^ n"
+          using hk by simp
+        have "top1_urysohn_U X TX U0 U1 (Suc n) k = top1_urysohn_U X TX U0 U1 n (k div (2::nat))"
+          using True by simp
+        thus ?thesis
+          using good_n hkdiv by blast
+      next
+        case False
+        have hkodd: "odd k" using False by simp
+        have hkdiv: "k div (2::nat) < (2::nat) ^ n"
+          using hk hkodd by simp
+        have hL: "top1_urysohn_U X TX U0 U1 n (k div (2::nat)) \<in> TX \<and> top1_urysohn_U X TX U0 U1 n (k div (2::nat)) \<subseteq> X"
+          using good_n hkdiv by blast
+        have hRidx: "Suc (k div (2::nat)) \<le> (2::nat) ^ n"
+          using hk hkodd by simp
+        have hR: "top1_urysohn_U X TX U0 U1 n (Suc (k div (2::nat))) \<in> TX \<and> top1_urysohn_U X TX U0 U1 n (Suc (k div (2::nat))) \<subseteq> X"
+          using good_n hRidx by blast
+        have hcl: "closure_on X TX (top1_urysohn_U X TX U0 U1 n (k div (2::nat)))
+            \<subseteq> top1_urysohn_U X TX U0 U1 n (Suc (k div (2::nat)))"
+          using step_n hkdiv by simp
+        show ?thesis
+          using step_odd[OF _ hkodd hL hR hcl] hk by blast
+      qed
+    qed
+
+    have step_Suc:
+      "\<forall>k<(2::nat) ^ Suc n. closure_on X TX (top1_urysohn_U X TX U0 U1 (Suc n) k)
+            \<subseteq> top1_urysohn_U X TX U0 U1 (Suc n) (Suc k)"
+    proof (intro allI impI)
+      fix k assume hk: "k < (2::nat) ^ Suc n"
+      show "closure_on X TX (top1_urysohn_U X TX U0 U1 (Suc n) k)
+            \<subseteq> top1_urysohn_U X TX U0 U1 (Suc n) (Suc k)"
+      proof (cases "even k")
+        case True
+        have hkdiv: "k div (2::nat) < (2::nat) ^ n"
+          using hk True by simp
+        have hk1odd: "odd (Suc k)"
+          using True by simp
+        have hL: "top1_urysohn_U X TX U0 U1 n (k div (2::nat)) \<in> TX \<and> top1_urysohn_U X TX U0 U1 n (k div (2::nat)) \<subseteq> X"
+          using good_n hkdiv by blast
+        have hR: "top1_urysohn_U X TX U0 U1 n (Suc (k div (2::nat))) \<in> TX \<and> top1_urysohn_U X TX U0 U1 n (Suc (k div (2::nat))) \<subseteq> X"
+          using good_n by (simp add: hkdiv)
+        have hcl: "closure_on X TX (top1_urysohn_U X TX U0 U1 n (k div (2::nat)))
+            \<subseteq> top1_urysohn_U X TX U0 U1 n (Suc (k div (2::nat)))"
+          using step_n hkdiv by simp
+        have hodd_props:
+          closure_on X TX (top1_urysohn_U X TX U0 U1 n ((Suc k) div (2::nat)))
+            \<subseteq> top1_urysohn_U X TX U0 U1 (Suc n) (Suc k)
+          using step_odd[OF _ hk1odd hL hR hcl] hk by blast
+        have hEq0: "(Suc k) div (2::nat) = k div (2::nat)"
+          using True by simp
+        have hEq1: "top1_urysohn_U X TX U0 U1 (Suc n) k = top1_urysohn_U X TX U0 U1 n (k div (2::nat))"
+          using True by simp
+        show ?thesis
+          using hodd_props hEq0 hEq1 by blast
+      next
+        case False
+        have hkodd: "odd k" using False by simp
+        have hkdiv: "k div (2::nat) < (2::nat) ^ n"
+          using hk hkodd by simp
+        have hL: "top1_urysohn_U X TX U0 U1 n (k div (2::nat)) \<in> TX \<and> top1_urysohn_U X TX U0 U1 n (k div (2::nat)) \<subseteq> X"
+          using good_n hkdiv by blast
+        have hRidx: "Suc (k div (2::nat)) \<le> (2::nat) ^ n"
+          using hk hkodd by simp
+        have hR: "top1_urysohn_U X TX U0 U1 n (Suc (k div (2::nat))) \<in> TX \<and> top1_urysohn_U X TX U0 U1 n (Suc (k div (2::nat))) \<subseteq> X"
+          using good_n hRidx by blast
+        have hcl: "closure_on X TX (top1_urysohn_U X TX U0 U1 n (k div (2::nat)))
+            \<subseteq> top1_urysohn_U X TX U0 U1 n (Suc (k div (2::nat)))"
+          using step_n hkdiv by simp
+        have hodd_props:
+          closure_on X TX (top1_urysohn_U X TX U0 U1 (Suc n) k)
+            \<subseteq> top1_urysohn_U X TX U0 U1 n (Suc (k div (2::nat)))
+          using step_odd[OF _ hkodd hL hR hcl] hk by blast
+        have hEq: "top1_urysohn_U X TX U0 U1 (Suc n) (Suc k) =
+            top1_urysohn_U X TX U0 U1 n (Suc k div (2::nat))"
+          by (simp add: hkodd)
+        have hEqdiv: "(Suc k) div (2::nat) = Suc (k div (2::nat))"
+          using hkodd by simp
+        show ?thesis
+          using hodd_props hEq hEqdiv by blast
+      qed
+    qed
+
+    show ?case
+      unfolding P_def using good_Suc step_Suc by blast
+  qed
+
+  show ?thesis
+    using hP unfolding P_def by blast
+qed
+*)
+
 (** from \S33 Theorem 33.1 (Urysohn lemma) [top1.tex:4382] **)
 theorem Theorem_33_1:
   fixes a b :: real
